# Winkelfunktionen
+ $e^x=\sum_{n=0}^∞ \frac{x^n}{n!}$ konvergiert für alle x∈ℂ
	+ $i^2=-1$
	+  $e^{ix}=\sum_{n=0}^∞ \frac{(ix)^n}{n!}=\sum_{n=0}^∞ \frac{(ix)^{2n}}{(2n)!} + \sum_{n=0}^∞ \frac{(ix)^{2n+1}}{(2n+1)!}=$
	+  $=\sum_{n=0}^∞ (-1)^n \frac{x^{2n}}{(2n)!} + i \sum_{n=0}^∞ (-1)^n \frac{x^{2n+1}}{(2n+1)!}=cos(x) + sin(x)$ 
		+ $\sum_{n=0}^∞ (-1)^n \frac{x^{2n}}{(2n)!}=cos(x)$	
		+ $\sum_{n=0}^∞ (-1)^n \frac{x^{2n+1}}{(2n+1)!}=sin(x)$
	+ $e^{ix}=cos(x) + isin(x)$
+ $sin(x)^2+cos(x)^2=1$
+ $|sin(x)|≤1$ und $|cos(x)|≤1$
+ $sin(-x)=-sin(x)$
	+ gerade Funktion
+ $cos(-x)=cos(x)$
	+ ungerade Funktion
+ $sin(x)$ und $cos(x)$ sind alternierende Reihen

### Additionstheoreme
+ $cos(x+/-y)=cos(x)*cos(y)-/+sin(x)*sin(y)$
	+ $cos(x+y)=cos(x)*cos(y)+sin(x)*sin(y)$
	+ $cos(x-y)=cos(x)*cos(y)-sin(x)*sin(y)$
		+ $cos(x)cos(y)=\frac{1}{2}(cos(x+y)+cos(x-y))$
		+ $sin(x)sin(y)=\frac{1}{2}(cos(x-y)-cos(x+y))$
+ $sin(x+/-y)=sin(x)*cos(y)-/+cos(x)*sin(y)$
	+ $sin(x+y)=sin(x)*cos(y)+cos(x)*sin(y)$
	+ $sin(x-y)=sin(x)*cos(y)-cos(x)*sin(y)$
		+ $sin(x)cos(y)=\frac{1}{2}(sin(x+y)+sin(x-y))$
		+ $cos(x)sin(y)=\frac{1}{2}(sin(x-y)-sin(x+y))$
